Batch processing: verify and extract everything

src/3d/ocaml/Batch.ml
@@ -1,0 +1,210 @@
+let code_of_exit = function
+  | Unix.WEXITED i
+  | Unix.WSIGNALED i
+  | Unix.WSTOPPED i
+    -> i
+
+let filename_concat = Printf.sprintf "%s/%s" 
+
+let filename_quote s = s
+
+let run_cmd_gen reconcat prog args =
+  let cmd = String.concat " " (prog :: args) in
+  print_endline (Printf.sprintf "Running: %s" cmd);
+  let args' = Array.of_list (if reconcat then prog :: args else args) in (* FIXME: WHY WHY WHY do I need to recons the prog in front of the args? *)
+  print_endline (Printf.sprintf "Length of args' is: %d" (Array.length args'));
+  let pid = Unix.create_process prog args' Unix.stdin Unix.stdout Unix.stderr in
+  let (_, res) = Unix.waitpid [] pid in
+  let res = code_of_exit res in
+  if res <> 0 then exit res
+
+let run_cmd = run_cmd_gen true
+
+(* paths *)
+let fstar_home = Sys.getenv "FSTAR_HOME"
+let kremlin_home = Sys.getenv "KREMLIN_HOME"
+let kremlib = filename_concat kremlin_home "kremlib"
+let qd_home = Sys.getenv "QD_HOME"
+let lowparse_home = filename_concat (filename_concat qd_home "src") "lowparse"
+let ddd_home = filename_concat (filename_concat qd_home "src") "3d"
+let ddd_prelude_home = filename_concat (filename_concat (filename_concat qd_home "src") "3d") "prelude"
+
+(* fix all directory separators of a file *)
+let fix_seps =
+  if Sys.win32
+  then Str.global_replace (Str.regexp "/") "\\\\"
+  else Str.global_replace (Str.regexp "\\") "/"
+
+(* copy a file *)
+let copy
+  source target
+=
+  let cp =
+    if Sys.win32
+    then (filename_concat ddd_home "cp.bat")
+    else "cp"
+  in
+  run_cmd cp [ fix_seps source; fix_seps target ]
+
+(* fstar.exe executable *)
+let fstar_exe = (filename_concat (filename_concat fstar_home "bin") "fstar.exe")
+
+(* krml: on Windows, needs to be copied into .exe *)
+let krml out_dir =
+  let rec aux exn = function
+    | [] -> if exn then failwith "no krml found" else ""
+    | (dir, file) :: q ->
+      let candidate = filename_concat dir file in
+      if Sys.file_exists candidate then candidate else aux exn q
+  in
+  let dir = kremlin_home in
+  let dir_bin = filename_concat dir "bin" in
+  if Sys.win32
+  then
+    let candidate =
+      aux false [
+        (dir_bin, "krml.exe"); (* binary package *)
+        (dir, "krml.exe");
+        (out_dir, "krml.exe"); (* has already been copied before *)
+      ]
+    in
+    if candidate <> ""
+    then candidate
+    else begin
+      let target = filename_concat out_dir "krml.exe" in
+      if Unix.has_symlink ()
+      then
+        let candidate = aux true [(dir, "krml")] in
+        Unix.symlink candidate target
+      else begin
+        (* Here, Windows cannot even read symlinks *)
+        let dir' = filename_concat (filename_concat dir "_build") "src" in
+        let candidate = aux true [(dir', "Kremlin.native")] in
+        copy candidate target
+      end;
+      target
+    end
+  else
+    aux true [(dir, "krml")]
+
+(* command lines *)
+let fstar_args0 = [
+  "--cache_checked_modules";
+  "--already_cached"; "FStar,LowStar,C.Spec.Loops,LowParse";
+  "--include"; lowparse_home;
+  "--include"; kremlib;
+  "--include"; ddd_prelude_home;
+  "--cmi";
+]
+
+let list_snoc q a =
+  q @ [a]
+
+let verify_and_extract_module
+  out_dir
+  (file, modul)
+: unit
+=
+  let fst_file = filename_concat out_dir (Printf.sprintf "%s.fst" modul) in
+  let fsti_file = Printf.sprintf "%si" fst_file in
+  let fstar_args =
+    "--odir" :: out_dir ::
+    fstar_args0
+  in
+  run_cmd fstar_exe (list_snoc fstar_args (fsti_file));
+  run_cmd fstar_exe (list_snoc fstar_args (fst_file));
+  let fstar_extract_args =
+    "--extract_module" :: modul ::
+    "--codegen" :: "Kremlin" ::
+    fstar_args
+  in
+  run_cmd fstar_exe (list_snoc fstar_extract_args (fst_file))
+
+let ends_with
+  sg suff
+= let len = String.length sg in
+  let len_suff = String.length suff in
+  len >= len_suff &&
+  String.sub sg (len - len_suff) len_suff = suff
+
+let is_krml
+  filename
+= ends_with filename ".krml"
+
+let all_krmls_in_dir
+  dir
+= let h = Unix.opendir dir in
+  let rec aux accu =
+    match
+      begin try
+        Some (Unix.readdir h)
+      with End_of_file -> None
+      end
+    with
+    | None -> accu
+    | Some entry ->
+      aux (if is_krml entry then (filename_concat dir entry :: accu) else accu)
+  in
+  let res = aux [] in
+  Unix.closedir h;
+  res
+
+let all_everparse_krmls =
+  all_krmls_in_dir ddd_prelude_home
+
+let produce_c_files
+  (out_dir: string)
+  (files_and_modules: (string * string) list)
+: unit
+= 
+  let krml_files = List.fold_left
+    (fun accu (_, modul) -> filename_concat out_dir (Printf.sprintf "%s.krml" modul) :: accu)
+    all_everparse_krmls
+    files_and_modules
+  in
+  let krml_args =
+    "-tmpdir" :: out_dir ::
+    "-skip-compilation" ::
+    "-bundle" :: "ResultOps=Prims,C.\\*,FStar.\\*,LowStar.\\*,LowParse.\\*,Prelude,Prelude.\\*,Actions,EverParse3d.\\*[rename=EverParse,rename-prefix]" ::
+    "-warn-error" :: "-9@4" ::
+    "-fnoreturn-else" ::
+    "-fparentheses" ::
+    "-fcurly-braces" ::
+    "-fmicrosoft" ::
+    "-header" :: filename_concat ddd_home "noheader.txt" ::
+    "-minimal" :: 
+    "-add-include" :: "EverParse:\"EverParseEndianness.h\"" ::
+    "-static-header" :: "Prelude.StaticHeader,LowParse.Low.Base,Prelude,Actions,ResultOps" ::
+    "-no-prefix" :: "LowParse.Slice" ::
+    "-no-prefix" :: "LowParse.Low.BoundedInt" ::
+    "-no-prefix" :: "EverParse3d.InputBuffer.Aux" ::
+    krml_files
+  in
+  (* the argument list is too long, so we need to go through an argument file *)
+  let argfile = filename_concat out_dir "kremlin_args.rsp" in
+  let h = open_out argfile in
+  let rec aux = function
+    | [] -> ()
+    | a :: q ->
+      output_string h (Printf.sprintf "%s\n" a);
+      aux q
+  in
+  aux krml_args;
+  close_out h;
+  let krml = krml out_dir in
+  print_endline (Printf.sprintf "KReMLin found at: %s" krml);
+  run_cmd krml [Printf.sprintf "@%s" argfile]
+
+let postprocess
+  (out_dir: string)
+  (files_and_modules: (string * string) list)
+: unit
+= (* produce the .checked and .krml files.
+     FIXME: modules can be processed in parallel *)
+  List.iter (verify_and_extract_module out_dir) files_and_modules;
+  (* produce the C files *)
+  produce_c_files out_dir files_and_modules;
+  (* copy ancillaries *)
+  copy (filename_concat ddd_home ".clang-format") out_dir;
+  copy (filename_concat ddd_home (Printf.sprintf "EverParseEndianness%s.h" (if Sys.win32 then "_Windows_NT" else ""))) (filename_concat out_dir "EverParseEndianness.h");
+  ()
