src/3d/Main.fst
@@ -78,7 +78,10 @@ let process_file (fn: string) : ML unit =
 
 let go () : ML unit =
   let files = Options.parse_cmd_line() in
-  List.iter process_file files
+  List.iter process_file files;
+  let out_dir = Options.get_output_dir () in
+  let files_and_modules = List.map (fun file -> (file, Options.get_module_name file)) files in
+  if Options.get_batch () then Batch.postprocess out_dir files_and_modules
 
 #push-options "--warn_error -272" //top-level effects are okay
 #push-options "--admit_smt_queries true" //explicitly not handling all exceptions, so that we can meaningful backtraces
