src/3d/Batch.fsti
@@ -1,0 +1,7 @@
+module Batch
+open FStar.All
+
+val postprocess
+  (out_dir: string)
+  (files_and_modules: list (string & string))
+: ML unit
