src/3d/cp.bat
@@ -1,0 +1,4 @@
+@echo off
+echo source: %1
+echo target: %2
+copy %1 %2
